feat(KSA): Init Mutation DoNotVersion

AwsCryptographicMaterialProviders/runtimes/java/src/testExamples/java/software/amazon/cryptography/example/hierarchy/mutations/DoNotVersionTest.java
@@ -7,50 +7,66 @@ import org.testng.annotations.Test;
 import software.amazon.cryptography.example.Fixtures;
 import software.amazon.cryptography.example.hierarchy.AdminProvider;
 import software.amazon.cryptography.example.hierarchy.CreateKeyExample;
+import software.amazon.cryptography.example.hierarchy.KeyStoreProvider;
+import software.amazon.cryptography.example.hierarchy.ValidateKeyStoreItem;
+import software.amazon.cryptography.keystore.KeyStore;
 import software.amazon.cryptography.keystoreadmin.KeyStoreAdmin;
 import software.amazon.cryptography.keystoreadmin.model.InitializeMutationInput;
 import software.amazon.cryptography.keystoreadmin.model.InitializeMutationOutput;
+import software.amazon.cryptography.keystoreadmin.model.KeyManagementStrategy;
 import software.amazon.cryptography.keystoreadmin.model.Mutations;
+import software.amazon.cryptography.keystoreadmin.model.SystemKey;
 import software.amazon.cryptography.keystoreadmin.model.UnsupportedFeatureException;
 
 public class DoNotVersionTest {
 
-  static final String testPrefix =
-    "mutations-initialize-mutation-do-not-version-java";
+  static final String testPrefix = "initialize-mutation-do-not-version-java-";
 
   @Test
-  public void DoNotVersionThrowsUnsupportedFeatureExceptionTest() {
-    Assert.assertThrows(
-      UnsupportedFeatureException.class,
-      () -> {
-        // Uncomment BK Creation if you need to re-create the test key
-        // String branchKeyId = CreateKeyExample.CreateKey(
-        //   Fixtures.TEST_KEYSTORE_NAME,
-        //   Fixtures.TEST_LOGICAL_KEYSTORE_NAME,
-        //   Fixtures.KEYSTORE_KMS_ARN,
-        //   testPrefix,
-        //   Fixtures.ddbClientWest2
-        // );
-        Mutations mutations = Mutations
-          .builder()
-          .TerminalKmsArn(MRK_ARN_WEST)
-          .build();
-
-        InitializeMutationInput initInput = InitializeMutationInput
-          .builder()
-          .Mutations(mutations)
-          .Identifier(testPrefix)
-          .DoNotVersion(true)
-          .build();
-        KeyStoreAdmin admin = AdminProvider.admin(
-          Fixtures.TEST_KEYSTORE_NAME,
-          Fixtures.TEST_LOGICAL_KEYSTORE_NAME,
-          Fixtures.ddbClientWest2
-        );
-        InitializeMutationOutput initOutput = admin.InitializeMutation(
-          initInput
-        );
-      }
+  public void DoNotVersion() {
+    final KeyStoreAdmin admin = AdminProvider.admin();
+    String branchKeyId = testPrefix + java.util.UUID.randomUUID().toString();
+    Assert.assertEquals(
+      branchKeyId,
+      CreateKeyExample.CreateKey(Fixtures.KEYSTORE_KMS_ARN, branchKeyId, admin),
+      "Creation of test BK failed."
+    );
+    SystemKey systemKey = MutationsProvider.KmsSystemKey();
+    KeyManagementStrategy strategy = AdminProvider.strategy(
+      Fixtures.kmsClientWest2
+    );
+    InitializeMutationInput initInput = InitializeMutationInput
+      .builder()
+      .Mutations(
+        MutationsProvider.defaultMutation(Fixtures.POSTAL_HORN_KEY_ARN)
+      )
+      .Identifier(branchKeyId)
+      .DoNotVersion(true)
+      .SystemKey(systemKey)
+      .Strategy(strategy)
+      .build();
+    InitializeMutationOutput initOutput = admin.InitializeMutation(initInput);
+    MutationsProvider.workMutation(
+      branchKeyId,
+      systemKey,
+      initOutput.MutationToken(),
+      strategy,
+      admin,
+      (short) 10
+    );
+    final KeyStore keyStore = KeyStoreProvider.keyStore();
+    final String version = ValidateKeyStoreItem.ValidateActiveItem(
+      branchKeyId,
+      keyStore
+    );
+    Assert.assertNotNull(version, "Active Item validation failed.");
+    Assert.assertTrue(
+      ValidateKeyStoreItem.ValidateVersionItem(branchKeyId, version, keyStore),
+      "Version validation failed."
+    );
+    Assert.assertTrue(
+      ValidateKeyStoreItem.ValidateBeaconItem(branchKeyId, keyStore),
+      "Beacon validation failed."
     );
   }
 }
